Expressions.v
@@ -1,5 +1,204 @@
-
+Require Import CContext.
+Require Import Types.
+Require Import String.
+Require Import Maps.
 
 (* at its core, everything in C can be modeled as a natural **)
 Definition CCore_Value :=
   nat.
+
+Inductive CCore_exp :=
+| CVal: CCore_Value -> CCore_exp
+| CAddr: string -> CCore_exp 
+| CVar: string -> CCore_exp
+| CPlus: CCore_exp -> CCore_exp -> CCore_exp
+| CMinus: CCore_exp -> CCore_exp -> CCore_exp
+| CMult: CCore_exp -> CCore_exp -> CCore_exp
+(* | CDiv: CCore_exp -> CCore_exp -> CCore_exp **)
+| CEq: CCore_exp -> CCore_exp -> CCore_exp
+| CLt: CCore_exp -> CCore_exp -> CCore_exp
+| CAnd: CCore_exp -> CCore_exp -> CCore_exp
+| CPtr: CCore_Value -> CCore_exp
+(* | CStruct: forall xl, struct xl -> string -> CCore_exp.
+ how do I do this? **)
+| CStruct: string -> string -> CCore_exp.
+
+Inductive C_exp :=
+| C_mod: C_exp -> C_exp -> C_exp (* a % b **)
+| C_u_plus: C_exp -> C_exp (* +a **)
+| C_u_min: C_exp -> C_exp (* -a **)
+| C_neq: C_exp -> C_exp -> C_exp (* a != b **)
+| C_gt: C_exp -> C_exp -> C_exp (* a > b **)
+| C_ge: C_exp -> C_exp -> C_exp (* a >= b **)
+| C_le: C_exp -> C_exp -> C_exp (*a <= b **)
+| C_not: C_exp -> C_exp (* !a **)
+| C_or: C_exp -> C_exp -> C_exp (* a || b **)
+| C_deref: CCore_Value -> C_exp -> C_exp (* A[b] **)
+| C_arrow: CCore_Value -> string -> C_exp
+| C_tern: C_exp -> C_exp -> C_exp -> C_exp (* a ? b : c **).
+
+Bind Scope Exp_scope with C_exp.
+Bind Scope Exp_scope with CCore_exp.
+Delimit Scope Exp_scope with Ccom.
+
+Notation "a '_[_' b '_]'"
+  := (C_mod a b) (at level 105, left associativity) : Exp_scope.
+
+Notation "a '_._' b"
+  := (CStruct a b) (at level 105, left associativity) : Exp_scope.
+
+Notation "a '_->_' b"
+  := (C_arrow a b) (at level 105, left associativity) : Exp_scope.
+
+Notation "'+_' a"
+  := (C_u_plus a) (at level 80) :  Exp_scope.
+
+Notation "'-_' a"
+  := (C_u_min a) (at level 80) : Exp_scope.
+
+Notation "'!_' a"
+  := (C_not a) (at level 80) : Exp_scope.
+
+Notation "'*_' a"
+  := (CPtr a) (at level 80) : Exp_scope.
+
+Notation "'&_' a"
+  := (CAddr a) (at level 80) : Exp_scope.
+
+Notation "a '_*_' b"
+  := (CMult a b) (at level 50, left associativity) : Exp_scope.
+
+Notation "a '_%_' b"
+  := (CMult a b) (at level 50, left associativity) : Exp_scope.
+
+Notation "a '_+_' b"
+  := (CPlus a b) (at level 50, left associativity) : Exp_scope.
+
+Notation "a '_-_' b"
+  := (CMinus a b) (at level 50, left associativity) : Exp_scope.
+
+Notation "a '_==_' b"
+  := (CEq a b) (at level 38, left associativity) : Exp_scope.
+
+Notation "a '_!=_' b"
+  := (C_neq a b) (at level 38, left associativity) : Exp_scope.
+
+Notation "a '_<_' b"
+  := (CLt a b) (at level 38, left associativity) : Exp_scope.
+
+Notation "a '_<=_' b"
+  := (C_le a b) (at level 38, left associativity) : Exp_scope.
+
+Notation "a '_>_' b"
+  := (C_gt a b) (at level 38, left associativity) : Exp_scope.
+
+Notation "a '_>=_' b"
+  := (C_ge a b) (at level 38, left associativity) : Exp_scope.
+
+Notation "a _&&_ b"
+  := (CAnd a b) (at level 25, left associativity) : Exp_scope.
+
+Notation "a _||_ b"
+  := (C_or a b) (at level 24, left associativity) : Exp_scope.
+
+Notation "a _?_ b _:_ c"
+  := (C_tern a b c) (at level 23, right associativity) : Exp_scope.
+
+Open Scope Exp_scope.
+Reserved Notation " ctx '>>' exp '>>>' exp'" (at level 40).
+Inductive E_eval : context -> CCore_exp -> CCore_exp -> Prop :=
+| E_Eval_Var_s: forall s st h ht ctx str n,
+    space s st h ht = ctx ->
+    lookup_s s st str = Some n ->
+    ctx >> CVar str >>> CVal n
+| E_Eval_Var_h: forall s st h ht ctx str n,
+    space s st h ht = ctx ->
+    lookup_h h ht str = Some n ->
+    ctx >> CVar str >>> CVal n
+| E_Eval_Addr_s: forall s st h ht ctx str addr,
+    space s st h ht = ctx ->
+    addr_s st str = Some addr ->
+    ctx >> &_ str >>> CVal addr
+| E_Eval_Addr_h: forall s st h ht ctx str addr,
+    space s st h ht = ctx ->
+    addr_h ht str = Some addr ->
+    ctx >> &_ str >>> CVal addr
+| E_Eval_Plus_l: forall ctx (expl expl' expr: CCore_exp),
+    ctx >> expl >>> expl' ->
+    ctx >> (expl _+_ expr) >>> (expl' _+_ expr)
+| E_Eval_Plus_r: forall ctx expl expr expr',
+    ctx >> expr >>> expr' ->
+    ctx >> (expl _+_ expr) >>> (expl _+_ expr')
+| E_Eval_Plus_c: forall ctx n1 n2,
+    ctx >>  ((CVal n1) _+_ (CVal n2)) >>> CVal (n1 + n2)
+| E_Eval_Min_l: forall ctx expl expl' expr,
+    ctx >> expl >>> expl' ->
+    ctx >> (expl _-_ expr) >>> (expl' _-_ expr)
+| E_Eval_Min_r: forall ctx expl expr expr',
+    ctx >> expr >>> expr' ->
+    ctx >> (expl _-_ expr) >>> (expl _-_ expr')
+| E_Eval_Min_c: forall ctx n1 n2,
+    ctx >> ((CVal n1) _-_ (CVal n2)) >>> CVal (n1 - n2)
+| E_Eval_Mult_l: forall ctx expl expl' expr,
+    ctx >> expl >>> expl' ->
+    ctx >> (expl _*_ expr) >>> (expl' _*_ expr)
+| E_Eval_Mult_r: forall ctx expl expr expr',
+    ctx >> expr >>> expr' ->
+    ctx >> (expl _*_ expr) >>> (expl _*_ expr')
+| E_Eval_Mult_c: forall ctx n1 n2,
+    ctx >> ((CVal n1) _*_ (CVal n2)) >>> CVal (n1 * n2)
+| E_Eval_Eq_l: forall ctx expl expl' expr,
+    ctx >> expl >>> expl' ->
+    ctx >> (expl _==_ expr) >>> (expl' _==_ expr)
+| E_Eval_Eq_r: forall ctx expl expr expr',
+    ctx >> expr >>> expr' ->
+    ctx >> (expl _==_ expr) >>> (expl _==_ expr')
+| E_Eval_Eq_c_tru: forall ctx n1 n2,
+    n1 = n2 -> 
+    ctx >> ((CVal n1) _==_ (CVal n2)) >>> CVal 0
+| E_Eval_Eq_c_fls: forall ctx n1 n2,
+    n1 <> n2 ->
+    ctx >> ((CVal n1) _==_ (CVal n2)) >>> CVal 1
+| E_Eval_Lt_l: forall ctx expl expl' expr,
+    ctx >> expl >>> expl' ->
+    ctx >> (expl _<_ expr) >>> (expl' _<_ expr)
+| E_Eval_Lt_r: forall ctx expl expr expr',
+    ctx >> expr >>> expr' ->
+    ctx >> (expl _<_ expr) >>> (expl _<_ expr')
+| E_Eval_Lt_c_tru: forall ctx n1 n2,
+    n1 < n2 -> 
+    ctx >> ((CVal n1) _<_ (CVal n2)) >>> CVal 0
+| E_Eval_Lt_c_fls: forall ctx n1 n2,
+    n1 >= n2 ->
+    ctx >> ((CVal n1) _<_ (CVal n2)) >>> CVal 1
+| E_Eval_And_l: forall ctx expl expl' expr,
+    ctx >> expl >>> expl' ->
+    ctx >> (expl _&&_ expr) >>> (expl' _&&_ expr)
+| E_Eval_And_r: forall ctx expl expr expr',
+    ctx >> expr >>> expr' ->
+    ctx >> (expl _&&_ expr) >>> (expl _&&_ expr')
+| E_Eval_And_c_tru: forall ctx n1 n2,
+    n1 = 0 /\ n2 = 0 -> 
+    ctx >> ((CVal n1) _&&_ (CVal n2)) >>> CVal 0
+| E_Eval_And_c_fls: forall ctx n1 n2,
+    n1 <> 0 \/ n2 <> 0 ->
+    ctx >> ((CVal n1) _&&_ (CVal n2)) >>> CVal 1
+| E_Eval_Ptr_s: forall s st h ht ctx ptr n,
+    space s st h ht = ctx ->
+    get_val_s s ptr = Some n ->
+    ctx >> *_ ptr >>> CVal n
+| E_Eval_Ptr_h: forall s st h ht ctx ptr n,
+    space s st h ht = ctx ->
+    get_val_h h ptr = Some n ->
+    ctx >> *_ ptr >>> CVal n
+| E_EVal_Struct_s: forall s st h ht ctx s_name s_var var val,
+    query_struct_space ctx s_name s_var = Some var ->
+    space s st h ht = ctx ->
+    lookup_s s st var = Some val ->
+    ctx >> (s_var _._ var) >>> CVal val
+
+where " ctx '>>' exp '>>>' exp'" := (E_eval ctx exp exp').
+
+    
+    
+  
